\documentclass[12pt,letterpaper]{article}
\usepackage[paperwidth=40cm,paperheight=150cm,left=10mm,right=1cm,top=2cm,bottom=2cm]{geometry}  % Adjust margins
\usepackage{amsmath}  % For math symbols and alignments
\usepackage{amsfonts} % For additional math fonts
\usepackage{amssymb}  % For symbols like \cdot

\begin{document} 
\begin{align*}
Input^{e}&=([Input_{ohe}]^{e}_{n_{W} \times n_V } \bullet [W_{emb}]_{n_V \times n_E})+P_e \\
Q_E&=Input^e \cdot Q_{e}; \quad K_E =Input^e \cdot K_{e}; \quad V_E=Input^e \cdot V_{e}\\
Ec_{t1}&=Norm(\sigma(\frac{Q_{E} K_{E}^T}{\sqrt d_k})V_{E}+Input^{e})=Norm(A_{e}+Input^{e})\\
FL_{e1}&=ReLu(Ec_{t1}*W^e_{fl_1}+b^e_{fl_1})\\
FL_{e2}&=FL_{e1}*W^e_{fl_2}+b^e_{fl_2}\\
Ec_{out}&=Norm(FL_{e2}+Ec_{t1})\\ \\
Input^{d}&=([Input_{ohe}]^{d}_{n_{W} \times n_V } \bullet [W_{emb}]_{n_V \times n_E})+P_e \\
Q_D&=Input^d \cdot Q_{d}\\
K_D&=Input^d \cdot K_{d}\\
V_D&=Input^d \cdot V_{d}\\
D_{t1}&=Norm(\sigma(Mask[\frac{Q_{D} K_{D}^T}{\sqrt d_k}])V_{D}+Input^{d})=Norm(A_{mask}+Input^d)\\
Q_C &= D_{t1} \cdot Q_{c}  \\
K_C &= Ec_{out} \cdot K_{c} \\
V_C &= Ec_{out} \cdot V_{c} \\
D_{t2} &= Norm\left(\sigma\left(\frac{Q_{C} K_{C}^T}{\sqrt{d_k}}\right) V_{C} + D_{t1}\right) = Norm(A_{cr}+D_{t1}) \\ %%Dt2
FL_{d1} &= ReLU(D_{t2} \cdot W^d_{fl_1} + b^d_{fl_1}) \\
FL_{d2} &= FL_{d1} \cdot W^d_{fl_2} + b^d_{fl_2} \\
D_{out} &= Norm(FL_{d2} + D_{t2}) =\frac{(FL_{d2} + D_{t2})-\mu_{(FL_{d2} + D_{t2})}}{\sqrt{\sigma^2_{(FL_{d2} + D_{t2})}+\epsilon}}\\
Z_{out} &= D_{out} \cdot W^o + b^o \\
\sigma(Z^{out}) &= \sigma(D_{out} \cdot W^o + b^o) 
\\\\%%%%%%%%%%%%%%%%%%%%%%%%%%%%%%%%%%%%%%%%%%%%%%%%%%%%%%%%%%%%%%%%%%%%%%%%%%%%%%%%%%%%%%%%%%%%%%%%%% FIRST
\frac{\partial \text{Loss}}{\partial Z^{out}} &= %% Z^{out}
\frac{\partial \text{Loss}}{\partial \sigma(Z^{out})} \cdot 
\frac{\partial \sigma(\partial Z^{out})}{\partial Z^{out}} = 
\sigma(Z^{out}_i) - y_i 
\\
\frac{\partial \text{Loss}}{\partial D_{out}} &= %% D^{{out}}
\frac{\partial \text{Loss}}{\partial \sigma(Z^{out})} \cdot 
\frac{\partial \sigma(\partial Z^{out})}{\partial Z^{out}} \cdot 
\frac{\partial Z^{out}}{\partial D_{out}} = (\sigma(Z^{out}_i) - y_i) \cdot W^o
\\
\frac{\partial \text{Loss}}{\partial W^{0}} &= %%     w^{0}
\frac{\partial \text{Loss}}{\partial Z^{out}} \cdot 
\frac{\partial Z^{out}}{\partial W^{0}}  = (\sigma(Z^{out}_i) - y_i) \cdot D_{out}
\\
\frac{\partial \text{Loss}}{\partial b^{0}} &= %%     b^{0}
\frac{\partial \text{Loss}}{\partial Z^{out}} \cdot 
\frac{\partial Z^{out}}{\partial b^{0}}  = (\sigma(Z^{out}_i) - y_i) \cdot 1
\\
\frac{\partial \text{Loss}}{\partial FL_{d2}} &= %% FL_{d2}
\frac{\partial \text{Loss}}{\partial \sigma(Z^{out})} \cdot 
\frac{\partial \sigma(\partial Z^{out})}{\partial Z^{out}} \cdot 
\frac{\partial Z^{out}}{\partial D_{out}} \cdot
\frac{\partial D_{out}}{\partial FL_{d2}} 
\\
\frac{\partial \text{Loss}}{\partial D_{t2}} &= %% D_{t2}
\frac{\partial \text{Loss}}{\partial \sigma(Z^{out})} \cdot 
\frac{\partial \sigma(\partial Z^{out})}{\partial Z^{out}} \cdot 
\frac{\partial Z^{out}}{\partial D_{out}} \cdot
\frac{\partial D_{out}}{\partial D_{t2}}
\\
\frac{\partial D_{out}}{\partial FL_{d2}}&=
\frac{\partial Norm(FL_{d2} + D_{t2})}{\partial FL_{d2}}=
\frac{\partial \frac{(FL_{d2} + D_{t2})-\mu_{(FL_{d2} + D_{t2})}}{\sqrt{\sigma^2_{(FL_{d2} + D_{t2})}+\epsilon}}}{\partial FL_{d2}}
\\\\
X&= FL_{d2} + D_{t2} ;\\ \\
\frac{\partial D_{out}}{\partial FL_{d2}}&=
\frac{\partial \frac{X-\mu_{(X)}}{\sqrt{\sigma^2_{(X)}+\epsilon}}}{\partial X}\cdot\frac{\partial X}{\partial FL_{d2}}
\\
\frac{\partial D_{out}}{\partial D_{t2}}&=
\frac{\partial \frac{X-\mu_{(X)}}{\sqrt{\sigma^2_{(X)}+\epsilon}}}{\partial X}\cdot\frac{\partial X}{\partial D_{t2}}
\\\\
\frac{\partial \frac{X-\mu_{(X)}}{\sqrt{\sigma^2_{(X)}+\epsilon}}}{\partial X} &=
\frac{\partial \frac{X-\mu_{(X)}}{\sqrt{\sigma^2_{(X)}+\epsilon}}}{\partial X}+
\frac{\partial \frac{X-\mu_{(X)}}{\sqrt{\sigma^2_{(X)}+\epsilon}}}{\partial \mu_{(X)}}\cdot \frac{\partial \mu_{(X)}}{\partial X}+
\frac{\partial \frac{X-\mu_{(X)}}{\sqrt{\sigma^2_{(X)}+\epsilon}}}{\partial \sigma^2_{(X)}}\cdot \frac{\partial \sigma^2_{(X)}}{\partial X}\\
\frac{\partial \frac{X-\mu_{(X)}}{\sqrt{\sigma^2_{(X)}+\epsilon}}}{\partial X} &=\frac{1}{\sqrt{\sigma^2_{(X)}+\epsilon}}\\
\frac{\partial \frac{X-\mu_{(X)}}{\sqrt{\sigma^2_{(X)}+\epsilon}}}{\partial \mu_{(X)}} \cdot \frac{\partial \mu_{(X)}}{\partial X } &=-\frac{1}{\sqrt{\sigma^2_{(X)}+\epsilon}}\cdot \frac{1}{N}\\\\
\sigma^2_{(X)}&=\frac{1}{N}\sum(X-\mu_{x})^2;\quad
\frac{\partial \sigma^2_{(X)}}{\partial X}=  \frac{2}{N}(X-\mu_{x})\cdot 1\\\\
\frac{\partial \frac{X-\mu_{(X)}}{\sqrt{\sigma^2_{(X)}+\epsilon}}}{\partial \sigma^2_{(X)}}\cdot \frac{\partial \sigma^2_{(X)}}{\partial X}&=
\frac{\partial}{\partial \sigma^2_{(X)}} \frac{X-\mu_{(X)}}{(\sigma^2_{(X)}+\epsilon)^{-1/2}}\cdot \frac{\partial \sigma^2_{(X)}}{\partial X}=
-\frac{1}{2}(\sigma^2_{(X)}+\epsilon)^{-3/2}\cdot 1 \cdot (X-\mu_{(X)})\frac{\partial \sigma^2_{(X)}}{\partial X}=
-\frac{1}{2}\frac{X-\mu_{(X)}}{(\sigma^2_{(X)}+\epsilon)^{3/2}}\cdot \frac{2}{N}(X-\mu_{x})\cdot 1=
-\frac{1}{N}\frac{(X-\mu_{(X)})^2}{(\sigma^2_{(X)}+\epsilon)^{3/2}}\\\\
\frac{\partial D_{out}}{\partial FL_{d2}}&=(1-\frac{1}{N}) \frac{1}{\sqrt{\sigma^2_{(X)}+\epsilon}}-\frac{1}{N}\frac{(X-\mu_{(X)})^2}{(\sigma^2_{(X)}+\epsilon)^{3/2}}=\frac{\partial D_{out}}{\partial D_{t2}} 
\\
\frac{\partial \text{Loss}}{\partial FL_{d2}} &= %%FL_{d2}
\frac{\partial \text{Loss}}{\partial \sigma(Z^{out})} \cdot 
\frac{\partial \sigma(\partial Z^{out})}{\partial Z^{out}} \cdot 
\frac{\partial Z^{out}}{\partial D_{out}} \cdot 
\frac{\partial D_{out}}{\partial FL_{d2}}=
\left[\sigma(Z^{out}_i) - y_i\right] \cdot 
W^o \cdot 
\left[(1-\frac{1}{N}) \frac{1}{\sqrt{\sigma^2_{(X)}+\epsilon}}-\frac{1}{N}\frac{(X-\mu_{(X)})^2}{(\sigma^2_{(X)}+\epsilon)^{3/2}}\right]
\\
\frac{\partial \text{Loss}}{\partial D_{t2}} &=  %%D_{t2}
\frac{\partial \text{Loss}}{\partial \sigma(Z^{out})} \cdot 
\frac{\partial \sigma(\partial Z^{out})}{\partial Z^{out}} \cdot 
\frac{\partial Z^{out}}{\partial D_{out}}\cdot 
\frac{\partial D_{out}}{\partial D_{t2}}
=\left[(\sigma(Z^{out}_i) - y_i\right] \cdot 
W^o \cdot 
\left[(1-\frac{1}{N}) \frac{1}{\sqrt{\sigma^2_{(X)}+\epsilon}}-\frac{1}{N}\frac{(X-\mu_{(X)})^2}{(\sigma^2_{(X)}+\epsilon)^{3/2}}\right]\\
\\\\
\frac{\partial \text{Loss}}{\partial FL_{d1}} &= %FDL1
\frac{\partial \text{Loss}}{\partial FL_{d2}} \cdot 
\frac{\partial FL_{d2}}{\partial FL_{d1}}=
\frac{\partial \text{Loss}}{\partial FL_{d2}}\cdot W^d_{fl2}
\\
\frac{\partial \text{Loss}}{\partial W^d_{fl2}} &= %W^d_{fl2}
\frac{\partial \text{Loss}}{\partial FL_{d2}} \cdot 
\frac{\partial FL_{d2}}{\partial W^d_{fl2}}=
\frac{\partial \text{Loss}}{\partial FL_{d2}}\cdot FL_{d1}
\\
\frac{\partial \text{Loss}}{\partial b^d_{fl2}} &= %B^d_{fl2}
\frac{\partial \text{Loss}}{\partial FL_{d2}} \cdot 
\frac{\partial FL_{d2}}{\partial b^d_{fl2}}=
\frac{\partial \text{Loss}}{\partial FL_{d2}}\cdot 1
\\\\
X_{1d}&=D_{t2} \cdot W^d_{fl_1} + b^d_{fl_1}
\\\\
\frac{\partial \text{Loss}}{\partial D_{t2}} &= %D_{t2}  ReLu
\frac{\partial \text{Loss}}{\partial FL_{d1}} \cdot
\frac{\partial FL_{d1}}{\partial ReLu(X_{1d})} \cdot
\frac{\partial ReLu(X_{1d})}{\partial X_{1d}} \cdot
\frac{\partial X_{1d}}{\partial D_{t2}}=
 \begin{cases}
    \frac{\partial \text{Loss}}{\partial FL_{d1}} \cdot W^d_{fl_1}, & X_{1d} > 0 \\
    0, & \text{otherwise}
    \end{cases} 
    \\
\frac{\partial \text{Loss}}{\partial W_{fl1}} &= %W_{fl1}
\frac{\partial \text{Loss}}{\partial FL_{d1}} \cdot
\frac{\partial FL_{d1}}{\partial ReLu(X_{1d} )} \cdot
\frac{\partial ReLu(X_{1d} )}{\partial X_{1d} } \cdot
\frac{\partial X_{1d} }{\partial W_{fl1}}=
 \begin{cases}
    \frac{\partial \text{Loss}}{\partial FL_{d1}} \cdot D_{t2}, & X_{1d} > 0 \\
    0, & \text{otherwise}
    \end{cases}\\
\frac{\partial \text{Loss}}{\partial b_{fl1}} &= %b_{fl1}
\frac{\partial \text{Loss}}{\partial FL_{d1}} \cdot
\frac{\partial FL_{d1}}{\partial ReLu(X_{1d} )} \cdot
\frac{\partial ReLu(X_{1d} )}{\partial X_{1d} } \cdot
\frac{\partial X_{1d} }{\partial b_{fl1}}=
 \begin{cases}
    \frac{\partial \text{Loss}}{\partial FL_{d1}} \cdot 1, & X_{1d} > 0 \\
    0, & \text{otherwise}
    \end{cases} 
\\%%%%%%%%%%%%%%%%%%%%%%%%%%%%%%%%%%%%%%%%%%%%%%%%%%%%%%%%%%%%%%%%%%%%%%%%%%%%%%%%%%%%%%%%%%%%%%%%%%%%%%%%%FIRST
\\ %%%%%%%%%%%%%%%%%%%%%%%%%%%%%%%%%%%%%%%%%%%%%%%%%%%%%%%%%%%%%%%%%%%%%%%%%%%%%%%%%%%%%%%SECOND
A_{cr}&=\sigma\left(\frac{Q_{C} K_{C}^T}{\sqrt{d_k}}\right) \cdot V_{C}
\\
Res&=A_{cr}+ D_{t1}
\\ \\
\frac{\partial \text{Loss}}{\partial A_{cr}} &= %A_cr
\frac{\partial \text{Loss}}{\partial D_{t2}} \cdot 
\frac{\partial D_{t2}}{\partial Norm(Res)} \cdot
\frac{\partial Norm(Res)}{\partial Res} \cdot
\frac{\partial  Res}{\partial A_{cr}}=\frac{\partial \text{Loss}}{\partial D_{t2}} \cdot 
\left[(1-\frac{1}{N}) \frac{1}{\sqrt{\sigma^2_{(Res)}+\epsilon}}-\frac{1}{N}\frac{(Res-\mu_{(Res)})^2}{(\sigma^2_{(Res)}+\epsilon)^{3/2}}\right] 
\\
\frac{\partial \text{Loss}}{\partial D_{t1}} &= %Dt1
\frac{\partial \text{Loss}}{\partial D_{t2}} \cdot 
\frac{\partial D_{t2}}{\partial Norm(A_{cr}+D_{t1})} \cdot
\frac{\partial Norm(A_{cr}+D_{t1})}{\partial (A_{cr}+D_{t1})} \cdot
\frac{\partial  (A_{cr}+D_{t1})}{\partial D_{t1}}
\\
\frac{\partial \text{Loss}}{\partial D^{qc}_{t1}} &= %Dt1 qc
\frac{\partial \text{Loss}}{\partial A_{cr}} \cdot 
\frac{\partial A_{cr}}{\partial Q_{C}}\cdot
\frac{\partial Q_{C}}{\partial D_{t1}}=
\frac{\partial \text{Loss}}{\partial A_{cr}}\cdot
\sigma\left(\frac{Q_{C} K_{C}^T}{\sqrt{d_k}}\right)\cdot \left[1-\sigma\left(\frac{Q_{C} K_{C}^T}{\sqrt{d_k}}\right)\right]\cdot
\frac{K_{C}^T}{\sqrt{d_k}}\cdot V_C \cdot Q_{c}
\\
\frac{\partial \text{Loss}}{\partial Q_{c}} &= %Qc
\frac{\partial \text{Loss}}{\partial A_{cr}} \cdot 
\frac{\partial A_{cr}}{\partial Q_{C}}\cdot
\frac{\partial Q_{C}}{\partial Q_{c}}=
\frac{\partial \text{Loss}}{\partial A_{cr}}\cdot
\sigma\left(\frac{Q_{C} K_{C}^T}{\sqrt{d_k}}\right)\cdot \left[1-\sigma\left(\frac{Q_{C} K_{C}^T}{\sqrt{d_k}}\right)\right]\cdot
\frac{K_{C}^T}{\sqrt{d_k}}\cdot V_C \cdot D_{t1}
\\
\frac{\partial \text{Loss}}{\partial K_{c}} &= %Kc
\frac{\partial \text{Loss}}{\partial A_{cr}} \cdot 
\frac{\partial A_{cr}}{\partial K_{C}}\cdot
\frac{\partial K_{C}}{\partial K_{c}}=
\frac{\partial \text{Loss}}{\partial A_{cr}}\cdot
\sigma\left(\frac{Q_{C} K_{C}^T}{\sqrt{d_k}}\right)\cdot \left[1-\sigma\left(\frac{Q_{C} K_{C}^T}{\sqrt{d_k}}\right)\right]\cdot
\frac{Q_{C}}{\sqrt{d_k}}\cdot V_C \cdot Ec_{out}
\\
\frac{\partial \text{Loss}}{\partial V_{c}} &= %Vc
\frac{\partial \text{Loss}}{\partial A_{cr}} \cdot 
\frac{\partial A_{cr}}{\partial V_{C}}\cdot
\frac{\partial V_{C}}{\partial V_{c}}=
\frac{\partial \text{Loss}}{\partial A_{cr}}\cdot
\sigma\left(\frac{Q_{C} K_{C}^T}{\sqrt{d_k}}\right)
\cdot Ec_{out}
\\
\frac{\partial \text{Loss}}{\partial Ec^K_{cout}} &= %Ecout K
\frac{\partial \text{Loss}}{\partial A_{cr}} \cdot 
\frac{\partial A_{cr}}{\partial K_{C}}\cdot
\frac{\partial K_{C}}{\partial Ec_{cout}}=
\frac{\partial \text{Loss}}{\partial A_{cr}}\cdot
\sigma\left(\frac{Q_{C} K_{C}^T}{\sqrt{d_k}}\right)\cdot \left[1-\sigma\left(\frac{Q_{C} K_{C}^T}{\sqrt{d_k}}\right)\right]\cdot
\frac{Q_{C}}{\sqrt{d_k}}\cdot V_C \cdot K_c
\\
\frac{\partial \text{Loss}}{\partial Ec^V_{cout}} &= %Ecout Vc
\frac{\partial \text{Loss}}{\partial A_{cr}} \cdot 
\frac{\partial A_{cr}}{\partial V_{C}}\cdot
\frac{\partial V_{C}}{\partial Ec_{cout}}=
\frac{\partial \text{Loss}}{\partial A_{cr}}\cdot
\sigma\left(\frac{Q_{C} K_{C}^T}{\sqrt{d_k}}\right)
\cdot V_c
\\
\frac{\partial \text{Loss}}{\partial Ec_{cout}} &= %Ecout tot
\frac{\partial \text{Loss}}{\partial Ec^K_{cout}}+
\frac{\partial \text{Loss}}{\partial Ec^V_{cout}}
\\\\ \\
A_{mask}&=\sigma(Mask[\frac{Q_{D} K_{D}^T}{\sqrt d_k}])V_{D}=\sigma( \frac{Q_{D} K_{D}^T}{\sqrt d_k}+Mask)V_{D}
\\
X_d&=Input^d+A_{masked}
\\\\
\frac{\partial \text{Loss}}{\partial A_{mask}} &= %A_mask
\frac{\partial \text{Loss}}{\partial D_{t1}}\cdot
\frac{\partial D_{t1}}{\partial Norm(X_d)}\cdot
\frac{\partial Norm(X_d)}{\partial A_{mask}}
\\
\frac{\partial \text{Loss}}{\partial input^d_{dt1}} &= %input_d
\frac{\partial \text{Loss}}{\partial D_{t1}}\cdot
\frac{\partial D_{t1}}{\partial Norm(X_d)}\cdot
\frac{\partial Norm(X_d)}{\partial input^d}
\\
\frac{\partial \text{Loss}}{\partial Q_{d}} &= %QD
\frac{\partial \text{Loss}}{\partial A_{mask}}\cdot
\frac{\partial A_{mask}}{\partial Q_{D}} \cdot
\frac{\partial Q_{D}}{\partial Q_{d}}=
\frac{\partial \text{Loss}}{\partial A_{mask}} \cdot 
\sigma( \frac{Q_{D} K_{D}^T}{\sqrt d_k}+Mask)\cdot \left[1-\sigma( \frac{Q_{D} K_{D}^T}{\sqrt d_k}+Mask)\right]\cdot 
\frac{ K_{D}^T}{\sqrt d_k} \cdot V_{D} \cdot Input^d
\\
\frac{\partial \text{Loss}}{\partial K_{d}} &= %KD
\frac{\partial \text{Loss}}{\partial A_{mask}}\cdot
\frac{\partial A_{mask}}{\partial K_{D}} \cdot
\frac{\partial K_{D}}{\partial K_{d}}=
\frac{\partial \text{Loss}}{\partial A_{mask}} \cdot 
\sigma( \frac{Q_{D} K_{D}^T}{\sqrt d_k}+Mask)\cdot \left[1-\sigma( \frac{Q_{D} K_{D}^T}{\sqrt d_k}+Mask)\right]\cdot 
\frac{ Q_{D}}{\sqrt d_k} \cdot V_{D} \cdot Input^d
\\
\frac{\partial \text{Loss}}{\partial V_{d}} &= %VD
\frac{\partial \text{Loss}}{\partial A_{mask}}\cdot
\frac{\partial A_{mask}}{\partial V_{D}} \cdot
\frac{\partial V_{D}}{\partial V_{d}}=
\frac{\partial \text{Loss}}{\partial A_{mask}} \cdot 
\sigma( \frac{Q_{D} K_{D}^T}{\sqrt d_k}+Mask)\cdot Input^d
\\
\frac{\partial \text{Loss}}{\partial input^q_d} &= %%input_d QD
\frac{\partial \text{Loss}}{\partial A_{mask}}\cdot
\frac{\partial A_{mask}}{\partial Q_{D}} \cdot
\frac{\partial Q_{D}}{\partial input_d}=
\frac{\partial \text{Loss}}{\partial A_{mask}} \cdot 
\sigma( \frac{Q_{D} K_{D}^T}{\sqrt d_k}+Mask)\cdot \left[1-\sigma( \frac{Q_{D} K_{D}^T}{\sqrt d_k}+Mask)\right]\cdot 
\frac{ K_{D}^T}{\sqrt d_k} \cdot V_{D} \cdot Q_d
\\
\frac{\partial \text{Loss}}{\partial input^k_d} &= %%input_d KD
\frac{\partial \text{Loss}}{\partial A_{mask}}\cdot
\frac{\partial A_{mask}}{\partial K_{D}} \cdot
\frac{\partial K_{D}}{\partial input_d}=
\frac{\partial \text{Loss}}{\partial A_{mask}} \cdot 
\sigma( \frac{Q_{D} K_{D}^T}{\sqrt d_k}+Mask)\cdot \left[1-\sigma( \frac{Q_{D} K_{D}^T}{\sqrt d_k}+Mask)\right]\cdot 
\frac{ Q_{D}}{\sqrt d_k} \cdot V_{D} \cdot K_d
\\
\frac{\partial \text{Loss}}{\partial input^v_d} &= %%input_d VD
\frac{\partial \text{Loss}}{\partial A_{mask}}\cdot
\frac{\partial A_{mask}}{\partial V_{D}} \cdot
\frac{\partial V_{D}}{\partial input_d}=
\frac{\partial \text{Loss}}{\partial A_{mask}} \cdot 
\sigma( \frac{Q_{D} K_{D}^T}{\sqrt d_k}+Mask)\cdot V_d
\\
\frac{\partial \text{Loss}}{\partial input_d} &= %%input_d tot
\frac{\partial \text{Loss}}{\partial input^q_d}+
\frac{\partial \text{Loss}}{\partial input^k_d}+
\frac{\partial \text{Loss}}{\partial input^v_d}+
\frac{\partial \text{Loss}}{\partial input^d_{dt1}}
\\
\frac{\partial \text{Loss}}{\partial W_{emb}} &= %% Wdemb input  
\frac{\partial \text{Loss}}{\partial input_d} \cdot
\frac{\partial input_d}{\partial W_{emb}}=
\frac{\partial \text{Loss}}{\partial input_d} \cdot
Input_d
\\\\\\
\\
\frac{\partial \text{Loss}}{\partial Ec_{cout}} &= %Ecout tot
\frac{\partial \text{Loss}}{\partial Ec^K_{cout}}+
\frac{\partial \text{Loss}}{\partial Ec^V_{cout}}
\\
X_{e2}&=FL_{e2}+Ec_{t1}
\\\\
\frac{\partial \text{Loss}}{\partial FL_{e2}} &= %FLe2
\frac{\partial \text{Loss}}{\partial Ec_{cout}}\cdot
\frac{\partial Ec_{cout}}{\partial Norm(X_{e2})}\cdot
\frac{\partial Norm(X_{e2})}{\partial FL_{e2}}=
\frac{\partial \text{Loss}}{\partial Ec_{cout}}\cdot
\left[(1-\frac{1}{N}) \frac{1}{\sqrt{\sigma^2_{(X_{e2})}+\epsilon}}-\frac{1}{N}\frac{(X_{e2}-\mu_{(X_{e2})})^2}{(\sigma^2_{(X_{e2})}+\epsilon)^{3/2}}\right] 
\\
\frac{\partial \text{Loss}}{\partial E^{n}c_{t1}} &= %Ect1
\frac{\partial \text{Loss}}{\partial Ec_{cout}}\cdot
\frac{\partial Ec_{cout}}{\partial Norm(X_{e2})}\cdot
\frac{\partial Norm(X_{e2})}{\partial Ec_{t1}}=
\frac{\partial \text{Loss}}{\partial Ec_{cout}}\cdot
\left[(1-\frac{1}{N}) \frac{1}{\sqrt{\sigma^2_{(X_{e2})}+\epsilon}}-\frac{1}{N}\frac{(X_{e2}-\mu_{(X_{e2})})^2}{(\sigma^2_{(X_{e2})}+\epsilon)^{3/2}}\right] 
\\
\frac{\partial \text{Loss}}{\partial W^e_{fl2}} &= %We fl2
\frac{\partial \text{Loss}}{\partial FL_{e2}}\cdot
\frac{\partial FL_{e2}}{\partial W^e_{fl2}}=
\frac{\partial \text{Loss}}{\partial FL_{e2}}\cdot Fl_{e1}
\\
\frac{\partial \text{Loss}}{\partial b^e_{fl2}} &= %be fl2
\frac{\partial \text{Loss}}{\partial FL_{e2}}\cdot
\frac{\partial FL_{e2}}{\partial b^e_{fl2}}=
\frac{\partial \text{Loss}}{\partial FL_{e2}}\cdot 1
\\ 
\frac{\partial \text{Loss}}{\partial FL_{e1}} &= %Fl_{e1}
\frac{\partial \text{Loss}}{\partial FL_{e2}}\cdot
\frac{\partial FL_{e2}}{\partial FL_{e1}}=
\frac{\partial \text{Loss}}{\partial Fl_{e2}}\cdot W^e_{fl2}
\\
\\
X_{e1}&=Ec_{t1}\cdot W^e_{fl_1}+b^e_{fl_1}
\\
\\
\frac{\partial \text{Loss}}{\partial E_{ct1}} &= %E_{ct1}
\frac{\partial \text{Loss}}{\partial FL_{e1}} \cdot
\frac{\partial FL_{e1}}{\partial ReLu(X_{e1})} \cdot
\frac{\partial ReLu(X_{e1})}{\partial X_{e1}} \cdot
\frac{\partial X_{e1}}{\partial Ec_{t1}}=
 \begin{cases}
    \frac{\partial \text{Loss}}{\partial FL_{e1}} \cdot W^e_{fl_1}, &  X_{e1} > 0 \\
    0, & \text{otherwise}
    \end{cases} \\
\\
\frac{\partial \text{Loss}}{\partial W^e_{fl1}} &= %W^e_{fl1}
\frac{\partial \text{Loss}}{\partial FL_{e1}} \cdot
\frac{\partial FL_{e1}}{\partial ReLu(X_{e1})} \cdot
\frac{\partial ReLu(X_{e1})}{\partial (X_{e1})} \cdot
\frac{\partial (X_{e1})}{\partial W^e_{fl1}}=
 \begin{cases}
    \frac{\partial \text{Loss}}{\partial FL_{e1}} \cdot Ec_{t1}, &  X_{e1} > 0 \\
    0, & \text{otherwise}
    \end{cases} \\ 
\\
\frac{\partial \text{Loss}}{\partial b^e_{fl1}} &= %b^e_{fl1}
\frac{\partial \text{Loss}}{\partial FL_{e1}} \cdot
\frac{\partial FL_{e1}}{\partial ReLu(X_{e1})} \cdot
\frac{\partial ReLu(X_{e1})}{\partial (X_{e1})} \cdot
\frac{\partial (X_{e1})}{\partial b^e_{fl1}}=
\begin{cases}
\frac{\partial \text{Loss}}{\partial FL_{e1}} \cdot1, &  X_{e1} > 0 \\
0, & \text{otherwise}
\end{cases} \\ 
\\
\\
A_{e}&=\sigma(\frac{Q_{E} K_{E}^T}{\sqrt d_k})V_{E}
\\
X_{e1}&=A_{e}+Input^{e}
\\
\\
\frac{\partial \text{Loss}}{\partial A_{e}} &= %Ae
\frac{\partial \text{Loss}}{\partial Ec_{t1}} \cdot 
\frac{\partial Ec_{t1}}{\partial Norm(X_{e1})} \cdot 
\frac{\partial Norm(X_{e1})}{\partial A_{e}}=
\frac{\partial \text{Loss}}{\partial E_{ct1}}\cdot 
\left[(1-\frac{1}{N}) \frac{1}{\sqrt{\sigma^2_{(X_{e1})}+\epsilon}}-\frac{1}{N}\frac{(X_{e1}-\mu_{(X_{e1})})^2}{(\sigma^2_{(X_{e1})}+\epsilon)^{3/2}}\right] 
\\
\frac{\partial \text{Loss}}{\partial Input^{e}_n} &= %inpute Norm
\frac{\partial \text{Loss}}{\partial Ec_{t1}} \cdot 
\frac{\partial Ec_{t1}}{\partial Norm(X_{e1})} \cdot 
\frac{\partial Norm(X_{e1})}{\partial Input^{e}} =
\frac{\partial \text{Loss}}{\partial E_{ct1}}\cdot 
\left[(1-\frac{1}{N}) \frac{1}{\sqrt{\sigma^2_{(X_{e1})}+\epsilon}}-\frac{1}{N}\frac{(X_{e1}-\mu_{(X_{e1})})^2}{(\sigma^2_{(X_{e1})}+\epsilon)^{3/2}}\right] 
\\
\frac{\partial \text{Loss}}{\partial K_{e}} &= %Ke
\frac{\partial \text{Loss}}{\partial A_{e}} \cdot 
\frac{\partial A_{e}}{\partial K_{E}}\cdot
\frac{\partial K_{E}}{\partial K_{e}}=
\frac{\partial \text{Loss}}{\partial A_{e}}\cdot
\sigma\left(\frac{Q_{E} K_{E}^T}{\sqrt{d_k}}\right)\cdot \left[1-\sigma\left(\frac{Q_{E} K_{E}^T}{\sqrt{d_k}}\right)\right]\cdot
\frac{Q_{E}}{\sqrt{d_k}}\cdot V_E \cdot Input^e
\\
\frac{\partial \text{Loss}}{\partial Q_{e}} &= %Qe
\frac{\partial \text{Loss}}{\partial A_{e}} \cdot 
\frac{\partial A_{e}}{\partial Q_{E}}\cdot
\frac{\partial Q_{E}}{\partial Q_{e}}=
\frac{\partial \text{Loss}}{\partial A_{e}}\cdot
\sigma\left(\frac{Q_{E} K_{E}^T}{\sqrt{d_k}}\right)\cdot \left[1-\sigma\left(\frac{Q_{E} K_{E}^T}{\sqrt{d_k}}\right)\right]\cdot
\frac{K_{E}^T}{\sqrt{d_k}}\cdot V_E \cdot Input^e
\\
\frac{\partial \text{Loss}}{\partial V_{e}} &= %VE
\frac{\partial \text{Loss}}{\partial A_{e}} \cdot 
\frac{\partial A_{e}}{\partial V_{E}}\cdot
\frac{\partial V_{E}}{\partial V_{e}}=
\frac{\partial \text{Loss}}{\partial A_{e}}\cdot
\sigma\left(\frac{Q_{E} K_{E}^T}{\sqrt{d_k}}\right)
\cdot Input^e
\\
\frac{\partial \text{Loss}}{\partial Input^{e}_Q} &= %input e Q
\frac{\partial \text{Loss}}{\partial A_{e}} \cdot 
\frac{\partial A_{e}}{\partial Q_{E}}\cdot
\frac{\partial Q_{E}}{\partial Input^{e}}=
\frac{\partial \text{Loss}}{\partial A_{e}}\cdot
\sigma\left(\frac{Q_{E} K_{E}^T}{\sqrt{d_k}}\right)\cdot \left[1-\sigma\left(\frac{Q_{E} K_{E}^T}{\sqrt{d_k}}\right)\right]\cdot
\frac{K_{E}^T}{\sqrt{d_k}}\cdot V_E \cdot Q_e
\\
\frac{\partial \text{Loss}}{\partial Input^{e}_K} &= %input e K
\frac{\partial \text{Loss}}{\partial A_{e}} \cdot 
\frac{\partial A_{e}}{\partial K_{E}}\cdot
\frac{\partial K_{E}}{\partial Input^{e}}=
\frac{\partial \text{Loss}}{\partial A_{e}}\cdot
\sigma\left(\frac{Q_{E} K_{E}^T}{\sqrt{d_k}}\right)\cdot \left[1-\sigma\left(\frac{Q_{E} K_{E}^T}{\sqrt{d_k}}\right)\right]\cdot
\frac{Q_{E}}{\sqrt{d_k}}\cdot V_E \cdot K_e
\\
\frac{\partial \text{Loss}}{\partial Input^{e}_V} &= %%input e V
\frac{\partial \text{Loss}}{\partial A_{e}} \cdot 
\frac{\partial A_{e}}{\partial V_{E}}\cdot
\frac{\partial V_{E}}{\partial Input^{e}}=
\frac{\partial \text{Loss}}{\partial A_{e}}\cdot
\sigma\left(\frac{Q_{E} K_{E}^T}{\sqrt{d_k}}\right)
\cdot V_e
\\
\frac{\partial \text{Loss}}{\partial Input^{e}} &= %input e Tot
\frac{\partial \text{Loss}}{\partial Input^{e}_n}+
\frac{\partial \text{Loss}}{\partial Input^{e}_V}+
\frac{\partial \text{Loss}}{\partial Input^{e}_K}+
\frac{\partial \text{Loss}}{\partial Input^{e}_Q}
\\
\frac{\partial \text{Loss}}{\partial W^e_{emb}} &= %% Wdemb input  
\frac{\partial \text{Loss}}{\partial input^e} \cdot
\frac{\partial input^e}{\partial W^e_{emb}}=
\frac{\partial \text{Loss}}{\partial input^e} \cdot
Input^e
\\
\\\\ \\
\end{align*} 
\end{document}
